<?xml version="1.0"?>
<rdf:RDF xmlns="http://w3id.org/semapv/vocab/semapv-terms.owl#"
     xml:base="http://w3id.org/semapv/vocab/semapv-terms.owl"
     xmlns:owl="http://www.w3.org/2002/07/owl#"
     xmlns:rdf="http://www.w3.org/1999/02/22-rdf-syntax-ns#"
     xmlns:xml="http://www.w3.org/XML/1998/namespace"
     xmlns:xsd="http://www.w3.org/2001/XMLSchema#"
     xmlns:rdfs="http://www.w3.org/2000/01/rdf-schema#"
     xmlns:skos="http://www.w3.org/2004/02/skos/core#"
     xmlns:terms="http://purl.org/dc/terms/">
    <owl:Ontology rdf:about="http://w3id.org/semapv/vocab/semapv-terms.owl">
        <owl:versionIRI rdf:resource="http://w3id.org/semapv/vocab/releases/2025-01-06/semapv-terms.owl"/>
    </owl:Ontology>
    


    <!-- 
    ///////////////////////////////////////////////////////////////////////////////////////
    //
    // Annotation properties
    //
    ///////////////////////////////////////////////////////////////////////////////////////
     -->

    


    <!-- http://purl.org/dc/terms/source -->

    <owl:AnnotationProperty rdf:about="http://purl.org/dc/terms/source"/>
    


    <!-- http://www.w3.org/2004/02/skos/core#altLabel -->

    <owl:AnnotationProperty rdf:about="http://www.w3.org/2004/02/skos/core#altLabel"/>
    


    <!-- http://www.w3.org/2004/02/skos/core#definition -->

    <owl:AnnotationProperty rdf:about="http://www.w3.org/2004/02/skos/core#definition"/>
    


    <!-- http://www.w3.org/2004/02/skos/core#example -->

    <owl:AnnotationProperty rdf:about="http://www.w3.org/2004/02/skos/core#example"/>
    


    <!-- http://www.w3.org/2004/02/skos/core#prefLabel -->

    <owl:AnnotationProperty rdf:about="http://www.w3.org/2004/02/skos/core#prefLabel"/>
    


    <!-- 
    ///////////////////////////////////////////////////////////////////////////////////////
    //
    // Classes
    //
    ///////////////////////////////////////////////////////////////////////////////////////
     -->

    


    <!-- https://w3id.org/semapv/vocab/BackgroundKnowledgeBasedMatching -->

    <owl:Class rdf:about="https://w3id.org/semapv/vocab/BackgroundKnowledgeBasedMatching">
        <rdfs:subClassOf rdf:resource="https://w3id.org/semapv/vocab/Matching"/>
        <terms:source rdf:resource="https://doi.org/10.1016/j.websem.2018.04.001"/>
        <skos:definition>A matching process that exploits background knowledge from external resources, commonly referred to as background knowledge resources. This approach is also known as indirect matching, BK-based matching or context-based matching.</skos:definition>
        <skos:example>A match between a subject A and an object B was established because they appear equivalent under consideration of externally provided background knowledge.</skos:example>
        <skos:prefLabel>background knowledge-based matching process</skos:prefLabel>
    </owl:Class>
    


    <!-- https://w3id.org/semapv/vocab/BlankNormalisation -->

    <owl:Class rdf:about="https://w3id.org/semapv/vocab/BlankNormalisation">
        <rdfs:subClassOf rdf:resource="https://w3id.org/semapv/vocab/Normalization"/>
        <terms:source rdf:resource="https://doi.org/10.1007/978-3-642-38721-0"/>
        <skos:definition>A normalization technique replacing all blank characters, such as space, tabulation, carriage return (or sequences of these) into a single blank character.</skos:definition>
        <skos:example>The string &apos;ontology  matching&apos; (two spaces between &apos;ontology&apos; and &apos;matching) becomes &apos;ontology matching&apos; (one space).</skos:example>
        <skos:prefLabel>blank normalisation</skos:prefLabel>
    </owl:Class>
    


    <!-- https://w3id.org/semapv/vocab/CardinalityFiltering -->

    <owl:Class rdf:about="https://w3id.org/semapv/vocab/CardinalityFiltering">
        <rdfs:subClassOf rdf:resource="https://w3id.org/semapv/vocab/MatchingPostProcessing"/>
        <skos:prefLabel>cardinality filtering</skos:prefLabel>
    </owl:Class>
    


    <!-- https://w3id.org/semapv/vocab/CaseNormalization -->

    <owl:Class rdf:about="https://w3id.org/semapv/vocab/CaseNormalization">
        <rdfs:subClassOf rdf:resource="https://w3id.org/semapv/vocab/Normalization"/>
        <terms:source rdf:resource="https://doi.org/10.1007/978-3-642-38721-0"/>
        <skos:definition>A normalization technique converting each alphabetic character in a string to their lower case counterpart.</skos:definition>
        <skos:example>The string &apos;Ontology&apos; is normalised to &apos;ontology&apos; (lower case).</skos:example>
        <skos:prefLabel>case normalization</skos:prefLabel>
    </owl:Class>
    


    <!-- https://w3id.org/semapv/vocab/CompositeMatching -->

    <owl:Class rdf:about="https://w3id.org/semapv/vocab/CompositeMatching">
        <rdfs:subClassOf rdf:resource="https://w3id.org/semapv/vocab/Matching"/>
        <skos:definition>A matching process based on multiple, possibly intertwined, matching approaches.</skos:definition>
        <skos:example>An ontology matching tool determines that a subject should be mapped to an object by employing a range of techniques, including lexical, semantic and structural.</skos:example>
        <skos:prefLabel>composite matching process</skos:prefLabel>
    </owl:Class>
    


    <!-- https://w3id.org/semapv/vocab/DiacriticsSuppression -->

    <owl:Class rdf:about="https://w3id.org/semapv/vocab/DiacriticsSuppression">
        <rdfs:subClassOf rdf:resource="https://w3id.org/semapv/vocab/Normalization"/>
        <terms:source rdf:resource="https://doi.org/10.1007/978-3-642-38721-0"/>
        <skos:definition>A normalization technique replacing diactritic signs (e.g. accents, hats) with their most frequent replacements.</skos:definition>
        <skos:example>The string &apos;Protégé&apos; is normalised to &apos;Protege&apos;.</skos:example>
        <skos:prefLabel>diacritics suppression</skos:prefLabel>
    </owl:Class>
    


    <!-- https://w3id.org/semapv/vocab/DigitSuppression -->

    <owl:Class rdf:about="https://w3id.org/semapv/vocab/DigitSuppression">
        <rdfs:subClassOf rdf:resource="https://w3id.org/semapv/vocab/Normalization"/>
        <terms:source rdf:resource="https://doi.org/10.1007/978-3-642-38721-0"/>
        <skos:definition>A normalization technique removing all numbers in a string. </skos:definition>
        <skos:example>The string &apos;ontology1&apos; becomes &apos;ontology&apos;.</skos:example>
        <skos:prefLabel>digit suppression</skos:prefLabel>
    </owl:Class>
    


    <!-- https://w3id.org/semapv/vocab/EditDistance -->

    <owl:Class rdf:about="https://w3id.org/semapv/vocab/EditDistance">
        <rdfs:subClassOf rdf:resource="https://w3id.org/semapv/vocab/StringBasedSimilarityMeasure"/>
        <terms:source rdf:resource="https://doi.org/10.1007/978-3-642-38721-0"/>
        <skos:prefLabel>edit distance</skos:prefLabel>
    </owl:Class>
    


    <!-- https://w3id.org/semapv/vocab/HammingDistance -->

    <owl:Class rdf:about="https://w3id.org/semapv/vocab/HammingDistance">
        <rdfs:subClassOf rdf:resource="https://w3id.org/semapv/vocab/StringBasedSimilarityMeasure"/>
        <terms:source rdf:resource="https://doi.org/10.1007/978-3-642-38721-0"/>
        <skos:prefLabel>hamming distance</skos:prefLabel>
    </owl:Class>
    


    <!-- https://w3id.org/semapv/vocab/InstanceBasedMatching -->

    <owl:Class rdf:about="https://w3id.org/semapv/vocab/InstanceBasedMatching">
        <rdfs:subClassOf rdf:resource="https://w3id.org/semapv/vocab/Matching"/>
        <terms:source rdf:resource="https://doi.org/10.1007/978-3-642-38721-0"/>
        <skos:definition>A matching process based on individual representations (or instances).</skos:definition>
        <skos:example>A match between a subject A and an object B was established because they share the same instances.</skos:example>
        <skos:prefLabel>instance-based matching process</skos:prefLabel>
    </owl:Class>
    


    <!-- https://w3id.org/semapv/vocab/LanguageBasedSimilarityMeasure -->

    <owl:Class rdf:about="https://w3id.org/semapv/vocab/LanguageBasedSimilarityMeasure">
        <rdfs:subClassOf rdf:resource="https://w3id.org/semapv/vocab/SimilarityMeasure"/>
        <terms:source rdf:resource="https://doi.org/10.1007/978-3-642-38721-0"/>
        <skos:prefLabel>language-based similarity measure</skos:prefLabel>
    </owl:Class>
    


    <!-- https://w3id.org/semapv/vocab/Lemmatization -->

    <owl:Class rdf:about="https://w3id.org/semapv/vocab/Lemmatization">
        <rdfs:subClassOf rdf:resource="https://w3id.org/semapv/vocab/Normalization"/>
        <terms:source rdf:resource="https://doi.org/10.1007/978-3-642-38721-0"/>
        <skos:definition>The process of reducing the different forms of a word to one single form.</skos:definition>
        <skos:prefLabel>lemmatization</skos:prefLabel>
    </owl:Class>
    


    <!-- https://w3id.org/semapv/vocab/LevenshteinEditDistance -->

    <owl:Class rdf:about="https://w3id.org/semapv/vocab/LevenshteinEditDistance">
        <rdfs:subClassOf rdf:resource="https://w3id.org/semapv/vocab/EditDistance"/>
        <terms:source rdf:resource="https://doi.org/10.1007/978-3-642-38721-0"/>
        <skos:prefLabel>levenshtein distance</skos:prefLabel>
    </owl:Class>
    


    <!-- https://w3id.org/semapv/vocab/LexicalMatching -->

    <owl:Class rdf:about="https://w3id.org/semapv/vocab/LexicalMatching">
        <rdfs:subClassOf rdf:resource="https://w3id.org/semapv/vocab/Matching"/>
        <skos:definition>A matching process based on a lexical comparison between one or more syntactic features of the subject with one or more syntactic features of the object.</skos:definition>
        <skos:example>The label of a subject entity matches to an exact synonym of an object entity.</skos:example>
        <skos:prefLabel>lexical matching process</skos:prefLabel>
    </owl:Class>
    


    <!-- https://w3id.org/semapv/vocab/LexicalSimilarityThresholdMatching -->

    <owl:Class rdf:about="https://w3id.org/semapv/vocab/LexicalSimilarityThresholdMatching">
        <rdfs:subClassOf rdf:resource="https://w3id.org/semapv/vocab/Matching"/>
        <skos:definition>A lexical matching process based on a minimum threshold of a score from a comparison based on a lexical similarity algorithm.</skos:definition>
        <skos:example>A match between a subject and an object was established because they had a Levenshtein score higher than 0.8.</skos:example>
        <skos:prefLabel>lexical similarity threshold-based matching process</skos:prefLabel>
    </owl:Class>
    


    <!-- https://w3id.org/semapv/vocab/LinkStripping -->

    <owl:Class rdf:about="https://w3id.org/semapv/vocab/LinkStripping">
        <rdfs:subClassOf rdf:resource="https://w3id.org/semapv/vocab/Normalization"/>
        <terms:source rdf:resource="https://doi.org/10.1007/978-3-642-38721-0"/>
        <skos:definition>A normalization technique replacing specific links between words, such as apostrophes, dashes, underscore, etc into dashes or blanks.</skos:definition>
        <skos:example>The string &apos;alzheimer&apos;s&apos; becomes &apos;alzheimers&apos;.</skos:example>
        <skos:prefLabel>link stripping</skos:prefLabel>
    </owl:Class>
    


    <!-- https://w3id.org/semapv/vocab/LogicalConsistencyFiltering -->

    <owl:Class rdf:about="https://w3id.org/semapv/vocab/LogicalConsistencyFiltering">
        <rdfs:subClassOf rdf:resource="https://w3id.org/semapv/vocab/MatchingPostProcessing"/>
        <skos:prefLabel>logical consistency filtering</skos:prefLabel>
    </owl:Class>
    


    <!-- https://w3id.org/semapv/vocab/LogicalReasoning -->

    <owl:Class rdf:about="https://w3id.org/semapv/vocab/LogicalReasoning">
        <rdfs:subClassOf rdf:resource="https://w3id.org/semapv/vocab/Matching"/>
        <skos:definition>A matching process based on the inferences made by a logical reasoner.</skos:definition>
        <skos:example>Two classes across ontologies are determined equivalent by an OWL reasoner such as ELK.</skos:example>
        <skos:prefLabel>logical reasoning matching process</skos:prefLabel>
    </owl:Class>
    


    <!-- https://w3id.org/semapv/vocab/ManualMappingCuration -->

    <owl:Class rdf:about="https://w3id.org/semapv/vocab/ManualMappingCuration">
        <rdfs:subClassOf rdf:resource="https://w3id.org/semapv/vocab/Matching"/>
        <skos:definition>An matching process that is performed by a human agent and is based on human judgement and domain knowledge.</skos:definition>
        <skos:example>A human curator determines that a subject should be mapped to an object by virtue of their domain expertise.</skos:example>
        <skos:prefLabel>manual mapping curation</skos:prefLabel>
    </owl:Class>
    


    <!-- https://w3id.org/semapv/vocab/Mapping -->

    <owl:Class rdf:about="https://w3id.org/semapv/vocab/Mapping">
        <skos:definition>A triple &lt;s,p,o&gt; comprising a subject entity s, an object entity o and a mapping predicate p.</skos:definition>
        <skos:example>The subject entity NCI:C9305 is mapped to the object entity ICD10:C80.9 using the skos:relatedMatch mapping predicate.</skos:example>
        <skos:prefLabel>mapping</skos:prefLabel>
    </owl:Class>
    


    <!-- https://w3id.org/semapv/vocab/MappingActivity -->

    <owl:Class rdf:about="https://w3id.org/semapv/vocab/MappingActivity">
        <skos:definition>A process that relates to the creation, confirmation, rejection or curation of a mapping.</skos:definition>
        <skos:example>Matching is a mapping activity that results in the creating of a mapping; mapping review is an activity that results in the confirmation of a mapping.</skos:example>
        <skos:prefLabel>mapping activity</skos:prefLabel>
    </owl:Class>
    


    <!-- https://w3id.org/semapv/vocab/MappingChaining -->

    <owl:Class rdf:about="https://w3id.org/semapv/vocab/MappingChaining">
        <rdfs:subClassOf rdf:resource="https://w3id.org/semapv/vocab/Matching"/>
        <skos:definition>A matching process based on the traversing of multiple mappings.</skos:definition>
        <skos:example>A match between a subject A and an object B was established because A was mapped to C, C was mapped to D and D was mapped to B.</skos:example>
        <skos:prefLabel>mapping chaining-based matching process</skos:prefLabel>
    </owl:Class>
    


    <!-- https://w3id.org/semapv/vocab/MappingInversion -->

    <owl:Class rdf:about="https://w3id.org/semapv/vocab/MappingInversion">
        <rdfs:subClassOf rdf:resource="https://w3id.org/semapv/vocab/Matching"/>
        <terms:source rdf:resource="https://mapping-commons.github.io/sssom/chaining_rules/"/>
        <skos:altLabel>mapping flipping</skos:altLabel>
        <skos:altLabel>mapping inversion</skos:altLabel>
        <skos:altLabel>mapping inverting</skos:altLabel>
        <skos:altLabel>semantic walk-backs</skos:altLabel>
        <skos:definition>A matching process based on the inverting or flipping of the subject with the object of a mapping in accordance with the semantics of the mapping predicate.</skos:definition>
        <skos:example>A broad match between a subject A and an object B using the skos:narrowMatch mapping relation was established because B was mapped to A using the skos:broadMatch mapping relation.</skos:example>
        <skos:prefLabel>mapping inversion-based matching process</skos:prefLabel>
    </owl:Class>
    


    <!-- https://w3id.org/semapv/vocab/MappingReview -->

    <owl:Class rdf:about="https://w3id.org/semapv/vocab/MappingReview">
        <rdfs:subClassOf rdf:resource="https://w3id.org/semapv/vocab/MappingActivity"/>
        <skos:definition>A process that is concerned with determining if a mapping “candidate” (otherwise determined) is reasonable/correct.</skos:definition>
        <skos:example>A match between a subject A and an object B was established elsewhere, and a human reviewer determined that the mapping is true (or false) based on an independent evaluation.</skos:example>
        <skos:prefLabel>mapping review</skos:prefLabel>
    </owl:Class>
    


    <!-- https://w3id.org/semapv/vocab/Matching -->

    <owl:Class rdf:about="https://w3id.org/semapv/vocab/Matching">
        <rdfs:subClassOf rdf:resource="https://w3id.org/semapv/vocab/MappingActivity"/>
        <skos:altLabel>matching operation</skos:altLabel>
        <skos:altLabel>matching task</skos:altLabel>
        <skos:definition>An process that results in a mapping between a subject and an object entity.</skos:definition>
        <skos:example>The label of a subject entity matches to an exact synonym of an object entity.</skos:example>
        <skos:prefLabel>matching process</skos:prefLabel>
    </owl:Class>
    


    <!-- https://w3id.org/semapv/vocab/MatchingPostProcessing -->

    <owl:Class rdf:about="https://w3id.org/semapv/vocab/MatchingPostProcessing">
        <rdfs:subClassOf rdf:resource="https://w3id.org/semapv/vocab/MappingActivity"/>
        <skos:definition>A process applied to a set of mappings, usually with the intention of changing it.</skos:definition>
        <skos:prefLabel>matching process post-processing</skos:prefLabel>
    </owl:Class>
    


    <!-- https://w3id.org/semapv/vocab/MatchingPreprocessing -->

    <owl:Class rdf:about="https://w3id.org/semapv/vocab/MatchingPreprocessing">
        <rdfs:subClassOf rdf:resource="https://w3id.org/semapv/vocab/MappingActivity"/>
        <skos:definition>A preliminary processing of inputs prior to performing matching.</skos:definition>
        <skos:prefLabel>matching process pre-processing</skos:prefLabel>
    </owl:Class>
    


    <!-- https://w3id.org/semapv/vocab/Normalization -->

    <owl:Class rdf:about="https://w3id.org/semapv/vocab/Normalization">
        <rdfs:subClassOf rdf:resource="https://w3id.org/semapv/vocab/MatchingPreprocessing"/>
        <terms:source rdf:resource="https://doi.org/10.1007/978-3-642-38721-0"/>
        <skos:definition>A family of preprocessing techniques for reducing strings to be compared to a common format.</skos:definition>
        <skos:prefLabel>normalization</skos:prefLabel>
    </owl:Class>
    


    <!-- https://w3id.org/semapv/vocab/PunctuationElemination -->

    <owl:Class rdf:about="https://w3id.org/semapv/vocab/PunctuationElemination">
        <rdfs:subClassOf rdf:resource="https://w3id.org/semapv/vocab/Normalization"/>
        <terms:source rdf:resource="https://doi.org/10.1007/978-3-642-38721-0"/>
        <skos:definition>A normalization technique removing all punctation characters from a string.</skos:definition>
        <skos:example>The string &apos;e.g.&apos; becomes &apos;eg&apos;.</skos:example>
        <skos:prefLabel>punctuation elimination</skos:prefLabel>
    </owl:Class>
    


    <!-- https://w3id.org/semapv/vocab/RegexRemoval -->

    <owl:Class rdf:about="https://w3id.org/semapv/vocab/RegexRemoval">
        <rdfs:subClassOf rdf:resource="https://w3id.org/semapv/vocab/Normalization"/>
        <skos:definition>A preprocessing method transforming a string by matching a regular expression and then removing that match.</skos:definition>
        <skos:example>The regex match “[ -]phenotype” is removed from the label field of the subject entity in the mapping.</skos:example>
        <skos:prefLabel>regex removal</skos:prefLabel>
    </owl:Class>
    


    <!-- https://w3id.org/semapv/vocab/RegexReplacement -->

    <owl:Class rdf:about="https://w3id.org/semapv/vocab/RegexReplacement">
        <rdfs:subClassOf rdf:resource="https://w3id.org/semapv/vocab/Normalization"/>
        <skos:definition>A preprocessing method transforming a string by matching a regular expression and then replacing that match with a specified substitution string.</skos:definition>
        <skos:example>The regex match “[ -]phenotype” is replaced by “-disease” for the label field of the subject entity in the mapping.</skos:example>
        <skos:prefLabel>regex replacement</skos:prefLabel>
    </owl:Class>
    


    <!-- https://w3id.org/semapv/vocab/SemanticSimilarityThresholdMatching -->

    <owl:Class rdf:about="https://w3id.org/semapv/vocab/SemanticSimilarityThresholdMatching">
        <rdfs:subClassOf rdf:resource="https://w3id.org/semapv/vocab/Matching"/>
        <skos:definition>A matching process based on a minimum threshold of a score from a comparison based on a semantic similarity algorithm.</skos:definition>
        <skos:example>A match between a subject and an object entity was established because they had a Jaccard score higher than 0.8 based on the set of (common) superclasses.</skos:example>
        <skos:prefLabel>semantic similarity threshold-based matching process</skos:prefLabel>
    </owl:Class>
    


    <!-- https://w3id.org/semapv/vocab/SimilarityMeasure -->

    <owl:Class rdf:about="https://w3id.org/semapv/vocab/SimilarityMeasure">
        <terms:source rdf:resource="https://doi.org/10.1007/978-3-642-38721-0"/>
        <skos:definition>A technique for determining a score that characterises the similarity between two entities.</skos:definition>
        <skos:prefLabel>similarity measure</skos:prefLabel>
    </owl:Class>
    


    <!-- https://w3id.org/semapv/vocab/StableMarriageFiltering -->

    <owl:Class rdf:about="https://w3id.org/semapv/vocab/StableMarriageFiltering">
        <rdfs:subClassOf rdf:resource="https://w3id.org/semapv/vocab/MatchingPostProcessing"/>
        <skos:prefLabel>stable marriage filtering</skos:prefLabel>
    </owl:Class>
    


    <!-- https://w3id.org/semapv/vocab/Stemming -->

    <owl:Class rdf:about="https://w3id.org/semapv/vocab/Stemming">
        <rdfs:subClassOf rdf:resource="https://w3id.org/semapv/vocab/Normalization"/>
        <skos:definition>The process of reducing a word to its word stem.</skos:definition>
        <skos:prefLabel>stemming</skos:prefLabel>
    </owl:Class>
    


    <!-- https://w3id.org/semapv/vocab/StopWordRemoval -->

    <owl:Class rdf:about="https://w3id.org/semapv/vocab/StopWordRemoval">
        <rdfs:subClassOf rdf:resource="https://w3id.org/semapv/vocab/Normalization"/>
        <terms:source rdf:resource="https://doi.org/10.1007/978-3-642-38721-0"/>
        <skos:definition>A preprocessing method transforming a string by removing a list of stop words.</skos:definition>
        <skos:example>The stop-words “of, and, is, a” are removed from the label field of the subject entity in the mapping.</skos:example>
        <skos:prefLabel>stop-word removal</skos:prefLabel>
    </owl:Class>
    


    <!-- https://w3id.org/semapv/vocab/StringBasedSimilarityMeasure -->

    <owl:Class rdf:about="https://w3id.org/semapv/vocab/StringBasedSimilarityMeasure">
        <rdfs:subClassOf rdf:resource="https://w3id.org/semapv/vocab/SimilarityMeasure"/>
        <terms:source rdf:resource="https://doi.org/10.1007/978-3-642-38721-0"/>
        <skos:definition>A similarity measure based on the comparison of strings.</skos:definition>
        <skos:prefLabel>string-based similarity measure</skos:prefLabel>
    </owl:Class>
    


    <!-- https://w3id.org/semapv/vocab/StringEquality -->

    <owl:Class rdf:about="https://w3id.org/semapv/vocab/StringEquality">
        <rdfs:subClassOf rdf:resource="https://w3id.org/semapv/vocab/StringBasedSimilarityMeasure"/>
        <terms:source rdf:resource="https://doi.org/10.1007/978-3-642-38721-0"/>
        <skos:definition>A string-based similarity measure which involves determining if two strings associated with mapping entities are equal.</skos:definition>
        <skos:prefLabel>string equality</skos:prefLabel>
    </owl:Class>
    


    <!-- https://w3id.org/semapv/vocab/StructuralMatching -->

    <owl:Class rdf:about="https://w3id.org/semapv/vocab/StructuralMatching">
        <rdfs:subClassOf rdf:resource="https://w3id.org/semapv/vocab/Matching"/>
        <terms:source rdf:resource="https://doi.org/10.1016/j.websem.2009.11.002"/>
        <rdfs:comment>Structural matching does not involve looking at &quot;values&quot; of properties.</rdfs:comment>
        <skos:example>A match between a subject and an object was established because of the similarity of their structural features, e.g., the number of direct property of a class.</skos:example>
        <skos:prefLabel>structural matching process</skos:prefLabel>
    </owl:Class>
    


    <!-- https://w3id.org/semapv/vocab/SubstringSimilarity -->

    <owl:Class rdf:about="https://w3id.org/semapv/vocab/SubstringSimilarity">
        <rdfs:subClassOf rdf:resource="https://w3id.org/semapv/vocab/StringBasedSimilarityMeasure"/>
        <terms:source rdf:resource="https://doi.org/10.1007/978-3-642-38721-0"/>
        <skos:prefLabel>substring similarity</skos:prefLabel>
    </owl:Class>
    


    <!-- https://w3id.org/semapv/vocab/SubstringTest -->

    <owl:Class rdf:about="https://w3id.org/semapv/vocab/SubstringTest">
        <rdfs:subClassOf rdf:resource="https://w3id.org/semapv/vocab/StringBasedSimilarityMeasure"/>
        <terms:source rdf:resource="https://doi.org/10.1007/978-3-642-38721-0"/>
        <skos:prefLabel>substring test</skos:prefLabel>
    </owl:Class>
    


    <!-- https://w3id.org/semapv/vocab/TermExtraction -->

    <owl:Class rdf:about="https://w3id.org/semapv/vocab/TermExtraction">
        <rdfs:subClassOf rdf:resource="https://w3id.org/semapv/vocab/Normalization"/>
        <terms:source rdf:resource="https://doi.org/10.1007/978-3-642-38721-0"/>
        <skos:altLabel>named entity recognition</skos:altLabel>
        <skos:prefLabel>term extraction</skos:prefLabel>
    </owl:Class>
    


    <!-- https://w3id.org/semapv/vocab/ThresholdFiltering -->

    <owl:Class rdf:about="https://w3id.org/semapv/vocab/ThresholdFiltering">
        <rdfs:subClassOf rdf:resource="https://w3id.org/semapv/vocab/MatchingPostProcessing"/>
        <skos:prefLabel>threshold filtering</skos:prefLabel>
    </owl:Class>
    


    <!-- https://w3id.org/semapv/vocab/TokenBasedDistance -->

    <owl:Class rdf:about="https://w3id.org/semapv/vocab/TokenBasedDistance">
        <rdfs:subClassOf rdf:resource="https://w3id.org/semapv/vocab/StringBasedSimilarityMeasure"/>
        <terms:source rdf:resource="https://doi.org/10.1007/978-3-642-38721-0"/>
        <skos:prefLabel>token-based distance</skos:prefLabel>
    </owl:Class>
    


    <!-- https://w3id.org/semapv/vocab/Tokenization -->

    <owl:Class rdf:about="https://w3id.org/semapv/vocab/Tokenization">
        <rdfs:subClassOf rdf:resource="https://w3id.org/semapv/vocab/Normalization"/>
        <terms:source rdf:resource="https://doi.org/10.1007/978-3-642-38721-0"/>
        <skos:prefLabel>tokenization</skos:prefLabel>
    </owl:Class>
    


    <!-- https://w3id.org/semapv/vocab/UnspecifiedMatching -->

    <owl:Class rdf:about="https://w3id.org/semapv/vocab/UnspecifiedMatching">
        <rdfs:subClassOf rdf:resource="https://w3id.org/semapv/vocab/Matching"/>
        <skos:definition>A matching process based on an unspecified comparison.</skos:definition>
        <skos:example>A mapping between a subject and an object was established, but it is no longer clear how or why.</skos:example>
        <skos:prefLabel>unspecified matching process</skos:prefLabel>
    </owl:Class>
    


    <!-- https://w3id.org/semapv/vocab/nGramSimilarity -->

    <owl:Class rdf:about="https://w3id.org/semapv/vocab/nGramSimilarity">
        <rdfs:subClassOf rdf:resource="https://w3id.org/semapv/vocab/StringBasedSimilarityMeasure"/>
        <terms:source rdf:resource="https://doi.org/10.1007/978-3-642-38721-0"/>
        <skos:prefLabel>ngram similarity</skos:prefLabel>
    </owl:Class>
</rdf:RDF>



<!-- Generated by the OWL API (version 4.5.29) https://github.com/owlcs/owlapi -->

